[Scheme] more top level proof work

compiler/scheme/proofs/scheme_compileCorrectScript.sml
@@ -1,26 +1,200 @@
-open preamble;
-open scheme_astTheory;
-open scheme_semanticsTheory;
-open scheme_to_cakeTheory;
-open scheme_to_cakeProofTheory;
-open primSemEnvTheory;
-open primTypesTheory;
-open ffiTheory;
-open semanticsTheory;
-open evaluateTheory;
-open evaluatePropsTheory;
-open semanticPrimitivesTheory;
-
-val _ = new_theory "scheme_compileCorrect";
+(*
+  Top-level semantic preservation proof for Scheme
+*)
+Theory scheme_compileCorrect
+Ancestors
+  scheme_ast scheme_semantics scheme_to_cake
+  scheme_to_cakeProof primSemEnv primTypes
+  ffi semantics evaluate evaluateProps
+  semanticPrimitives scheme_to_cake_env
+  evaluate_dec ml_prog ast namespace
+  scheme_semanticsProps
+Libs
+  preamble
 
 (* avoid wasting time printing *)
-val _  = (max_print_depth := 15);
+val _  = (max_print_depth := 30);
+
+Theorem scheme_init_evaluate_dec:
+  ! ffi . ∃ ck1 ck2.
+    evaluate_decs (init_state ffi with clock := ck1) init_env
+      scheme_init =
+    (scheme_to_cake_env_st_1 ffi with clock := ck2,
+     Rval scheme_to_cake_env_env_13)
+Proof
+  `IS_SOME (check_cons_dec_list init_env.c scheme_init)`
+    by (EVAL_TAC >> simp[init_env_def] >> EVAL_TAC)
+  >> simp[GSYM evaluate_dec_list_eq_evaluate_decs]
+  >> simp[evaluate_decs_scheme_init_thm]
+QED
 
 Definition v_to_string_def:
   v_to_string (SBool F) = IO_event (ExtCall "scheme_out") (MAP (n2w o ORD) "#f") [] /\
   v_to_string (SBool T) = IO_event (ExtCall "scheme_out") (MAP (n2w o ORD) "#t") [] /\
   v_to_string _ = IO_event (ExtCall "scheme_out") (MAP (n2w o ORD) "other") []
 End
+
+Theorem every_one_con_check:
+  (! prog k .
+    every_exp
+      (one_con_check scheme_cons_env)
+      (cps_transform prog k)) /\
+  (! tfn ts es k .
+    every_exp (one_con_check scheme_cons_env) tfn /\
+    EVERY (every_exp (one_con_check scheme_cons_env)) ts
+    ==>
+    every_exp
+      (one_con_check scheme_cons_env)
+      (cps_transform_app tfn ts es k)) /\
+  (! xts bs e k .
+    EVERY (every_exp (one_con_check scheme_cons_env)) (MAP SND xts)
+    ==>
+    every_exp
+      (one_con_check scheme_cons_env)
+      (cps_transform_letinit xts bs e k)) /\
+  (! k es e .
+    every_exp
+      (one_con_check scheme_cons_env)
+      (cps_transform_seq k es e))
+Proof
+  simp [scheme_cons_env_simp]
+  >> ho_match_mp_tac cps_transform_ind
+  >> rpt strip_tac
+  >> simp[cps_transform_def]
+  >- (
+    Cases_on `v`
+    >> simp[lit_to_ml_val_def, do_con_check_def, nsLookup_def]
+    >- (
+      Cases_on `p`
+      >> simp[do_con_check_def, nsLookup_def]
+    )
+    >> Cases_on `b`
+    >> simp[do_con_check_def, nsLookup_def]
+  )
+  >> simp[refunc_set_def, do_con_check_def, nsLookup_def]
+  >- (
+    Induct_on `xs` >- (
+      Cases_on `xp`
+      >> simp[proc_ml_def, do_con_check_def, nsLookup_def]
+    )
+    >> simp[proc_ml_def, do_con_check_def, nsLookup_def]
+  )
+  >- (
+    rename1 `letpreinit_ml _ exp`
+    >> Induct_on `bs`
+    >> simp[letpreinit_ml_def, do_con_check_def, nsLookup_def]
+  )
+  >- (
+    gvs[cps_transform_def]
+    >> rename1 `letpreinit_ml _ exp`
+    >> Induct_on `bs`
+    >> simp[letpreinit_ml_def, do_con_check_def, nsLookup_def]
+  )
+  >-(
+    Induct_on `ts` using SNOC_INDUCT
+    >> simp[cons_list_def, do_con_check_def, nsLookup_def, REVERSE_SNOC]
+  )
+  >> Induct_on `xts`
+  >> simp[letinit_ml_def, do_con_check_def, nsLookup_def]
+  >> PairCases
+  >> simp[letinit_ml_def, do_con_check_def, nsLookup_def]
+QED
+
+Theorem scheme_semantics_preservation_terminates:
+  ! prog cml_prog v st env (ffi :'ffi ffi_state) .
+    scheme_semantics_prog prog (STerminate v) /\
+    static_scope_check prog = INR prog /\
+    codegen prog = INR cml_prog
+    ==>
+    semantics_prog (init_state ffi) init_env cml_prog (Terminate Success [v_to_string v])
+Proof
+  simp[semantics_prog_def, scheme_semantics_prog_def]
+  >> simp[static_scope_check_def]
+  >> simp_tac std_ss [codegen_def]
+  >> simp[evaluate_prog_with_clock_def]
+  >> rpt strip_tac
+  >> qspec_then `ffi` assume_tac scheme_init_evaluate_dec
+  >> gvs[]
+  >> qrefine `ck1 + k`
+  >> gvs[scheme_init_def]
+  >> simp[Once evaluate_decs_append]
+  >> dxrule_then assume_tac evaluate_decs_add_to_clock
+  >> gvs[]
+  >> pop_assum kall_tac
+  >> simp[Ntimes evaluate_decs_def 2]
+  >> simp[compile_scheme_prog_def]
+  >> simp[pat_bindings_def]
+  >> simp[extend_dec_env_def]
+  >> simp[Once scheme_init_env_defs]
+  >> simp[Once scheme_init_env_defs]
+  >> simp[Once scheme_init_env_defs]
+  >> simp[Once scheme_init_env_defs]
+  >> simp[Once scheme_init_env_defs]
+  >> simp[Once scheme_init_env_defs]
+  >> simp[Once scheme_init_env_defs]
+  >> simp[Once scheme_init_env_defs]
+  >> simp[Once scheme_init_env_defs]
+  >> simp[Once scheme_init_env_defs]
+  >> simp[Once scheme_init_env_defs]
+  >> simp[Once scheme_init_env_defs]
+  >> simp[GSYM scheme_cons_env_def]
+  >> simp[every_one_con_check]
+
+  >> simp[GSYM merge_env_def]
+  >> simp[GSYM scheme_to_cake_env_def]
+  >> simp[pmatch_def]
+  >> simp[Ntimes evaluate_def 2, nsOptBind_def]
+
+  >> gvs[scheme_semanticsTheory.steps_def]
+  >> drule_then assume_tac value_terminating
+  >> gvs[Once cont_rel_cases, Once valid_state_cases]
+  >> gvs[Once valid_cont_cases, can_lookup_cases, FEVERY_FEMPTY]
+  >> gvs[Once cps_rel_cases]
+  >> qmatch_goalsub_abbrev_tac `evaluate _ newenv [_]`
+  >> first_x_assum $ qspecl_then [`scheme_to_cake_env_st_1 ffi`, `newenv`] assume_tac
+  >> unabbrev_all_tac
+  >> gvs[scheme_init_st_defs]
+  >> gvs[scheme_env_sub, scheme_runtime_funs_def, basis_scheme_env]
+  >> Cases_on `ck2 <= ck`
+  >>> HEADGOAL (
+    qexists `ck - ck2`
+    >> simp[Once ADD_COMM]
+  )
+  >>> LASTGOAL (
+    qexists `0`
+    >> simp[]
+    >> dxrule_then assume_tac evaluate_add_to_clock
+    >> gvs[]
+    >> pop_assum $ qspec_then `ck2 - ck` assume_tac
+    >> gvs[]
+  )
+  >> simp[Ntimes evaluate_decs_def 2]
+  >> simp[pat_bindings_def]
+  >> `nsAppend scheme_to_cake_env_env_13.c init_env.c = scheme_cons_env` by (
+    simp[Once scheme_init_env_defs]
+    >> simp[Once scheme_init_env_defs]
+    >> simp[Once scheme_init_env_defs]
+    >> simp[Once scheme_init_env_defs]
+    >> simp[Once scheme_init_env_defs]
+    >> simp[Once scheme_init_env_defs]
+    >> simp[Once scheme_init_env_defs]
+    >> simp[Once scheme_init_env_defs]
+    >> simp[Once scheme_init_env_defs]
+    >> simp[Once scheme_init_env_defs]
+    >> simp[Once scheme_init_env_defs]
+    >> simp[Once scheme_init_env_defs]
+    >> simp[GSYM scheme_cons_env_def]
+  )
+  >> simp[scheme_cons_env_simp]
+  >> gvs[Once ml_v_vals_cases]
+  >~ [`bool_val_rel b mlb`] >>> HEADGOAL $ gvs[Once bool_val_rel_cases]
+  >> simp[Ntimes evaluate_def 2]
+  >> simp[evaluate_match_def, can_pmatch_all_def, pmatch_def,
+    nsLookup_def, same_type_def, same_ctor_def, pat_bindings_def]
+  >> simp[Ntimes evaluate_def 4, do_app_def, store_alloc_def, store_lookup_def,
+    EL_APPEND_EQN, call_FFI_def, store_assign_def, store_v_same_type_def]
+  >> cheat (*seems to depend on the ffi oracle here*)
+QED
 
 Theorem imp_semantics_prog:
   evaluate_decs (st with clock := ck) env p = (st1, Rval r) ∧
@@ -31,54 +205,7 @@ Proof
   \\ qexists_tac ‘ck’ \\ simp []
 QED
 
-Definition start_up_def:
-  start_up = scheme_basis_types ++ scheme_basis ++
-             [scheme_basis_list; scheme_basis_app]
-End
-
-fun abbrev_conv name tm =
-  let
-    val v = mk_var(name,type_of tm)
-    val def = new_definition(name ^ "_def", mk_eq(v, tm))
-  in
-    SYM def
-  end
-
-Theorem evaluate_decs_start_up =
-  “evaluate_decs
-     (FST (THE (prim_sem_env ffi)) with clock := ck)
-     (SND (THE (prim_sem_env ffi)))
-     start_up”
-  |> (SCONV [prim_sem_env_eq] THENC EVAL)
-  |> CONV_RULE (PATH_CONV "rrrlrr" (abbrev_conv "brack_env_v"))
-  |> CONV_RULE (PATH_CONV "rrrrlrr" (abbrev_conv "brack_env_c"))
-
-val brack_env_c_def = definition "brack_env_c_def";
-
-Definition brack_env_def:
-  brack_env = <|v := brack_env_v; c := brack_env_c|>
-End
-
-Theorem every_one_con_check:
-  every_exp
-    (one_con_check
-     (<| v := brack_env_v; c := brack_env_c|> +++
-              SND (THE (prim_sem_env st'.ffi))).c)
-     (cps_transform prog "k")
-Proof
-  simp [semanticPrimitivesTheory.extend_dec_env_def]
-  \\ rewrite_tac [prim_sem_env_eq, brack_env_def,
-                  LIST_CONJ (TypeBase.accessors_of “:'a sem_env”)]
-  \\ simp [namespaceTheory.nsAppend_def,brack_env_c_def]
-  \\ cheat (* proving the compiler doesn't produce bas conses *)
-QED
-
-Theorem steps_eq_FUNPOW_step:
-  ∀n s. steps n s = FUNPOW step n s
-Proof
-  Induct \\ simp [Once steps_def,FUNPOW]
-QED
-
+(*
 Theorem scheme_imp_cake:
   codegen prog = INR cake_code ∧
   static_scope ∅ prog ∧
@@ -129,6 +256,7 @@ Proof
   \\ gvs [Abbr‘e’,every_one_con_check]
   \\ cheat (* not too bad *)
 QED
+*)
 
 
 (*
@@ -215,4 +343,3 @@ QED
 *)
 
 val _  = (max_print_depth := 0); (* don't print stuff in docs *)
-val _ = export_theory();
